Done

src/Init/Data/String/Lemmas/Pattern/String/KMP.lean
@@ -7,9 +7,22 @@ module
 
 prelude
 public import Init.Data.String.Lemmas.Pattern.String.Basic
--- import Init.Data.ByteArray.Lemmas
-import Init.Omega
-import Init.ByCases
+public import Init.Data.String.Pattern.String
+import all Init.Data.String.Pattern.String
+import Init.Data.String.Lemmas.IsEmpty
+import Init.Data.Vector.Lemmas
+import Init.Data.Iterators.Lemmas.Basic
+import Init.Data.Iterators.Lemmas.Consumers.Collect
+import Init.Data.String.Lemmas.Basic
+import Init.Data.String.OrderInstances
+
+/-!
+# Verification of KMP string search
+
+In this file, we instantiate `LawfulToForwardSearcherModel` for `Slice` patterns, which amounts to
+verifying that our implementation of KMP string search in `Init.Data.String.Pattern.String` is
+correct.
+-/
 
 namespace String.Slice.Pattern
 
@@ -39,21 +52,14 @@ theorem partialMatch_add_one_add_one_iff {pat s : ByteArray} {stackPos needlePos
       PartialMatch pat s needlePos stackPos ∧ ∃ h₁ h₂, pat[needlePos]'h₁ = s[stackPos]'h₂ := by
   refine ⟨fun ⟨h₁, h₂, h₃, h₄⟩ => ?_, fun ⟨⟨h₁, h₂, h₃, h₄⟩, ⟨h₅, h₆, h₇⟩⟩ => ?_⟩
   · refine ⟨⟨by omega, by omega, by omega, fun j hj => ?_⟩, ⟨by omega, by omega, ?_⟩⟩
-    · rw [h₄ _ (by omega)]
-      congr 1
-      omega
-    · rw [h₄ _ (by omega)]
-      congr 1
-      omega
+    · simp [h₄ j (by omega), Nat.add_sub_add_right]
+    · simp [h₄ needlePos (by omega), Nat.add_sub_add_right,
+        Nat.sub_add_cancel (Nat.add_le_add_iff_right.1 h₃)]
   · refine ⟨by omega, by omega, by omega, fun j hj => ?_⟩
     by_cases hj' : j < needlePos
-    · rw [h₄ _ hj']
-      congr 1
-      omega
+    · simp [h₄ _ hj', Nat.add_sub_add_right]
     · obtain rfl : j = needlePos := by omega
-      rw [h₇]
-      congr 1
-      omega
+      simp [h₇, Nat.add_sub_add_right, h₃]
 
 theorem PartialMatch.partialMatch_of_le {pat s : ByteArray} {stackPos needlePos : Nat}
     (h : PartialMatch pat s needlePos stackPos) (newStackPos : Nat) (h' : newStackPos ≤ stackPos)
@@ -64,6 +70,11 @@ theorem PartialMatch.partialMatch_of_le {pat s : ByteArray} {stackPos needlePos 
   congr 1
   omega
 
+/--
+This is the key lemma for the correctness of KMP. Given a partial match of `pat` in `s`, it shows
+that all shorter partial matches of `pat` in `s` ending at the same position are described by
+partial matches of `pat` in itself.
+-/
 theorem PartialMatch.partialMatch_iff {pat s : ByteArray} {stackPos needlePos : Nat}
     (h : PartialMatch pat s needlePos stackPos) {needlePos' : Nat} :
     PartialMatch pat pat needlePos' needlePos ↔
@@ -86,9 +97,47 @@ theorem matchesAt_iff_partialMatch {pat s : Slice} (hpat : pat.isEmpty = false) 
   refine ⟨fun ⟨h, h'⟩ => ⟨h, Nat.le_refl _, by simp, fun j hj => by simp [h' j hj]⟩, fun h => ?_⟩
   exact ⟨h.stackPos_le_size, fun j hj => by simp [h.getElem_eq j hj]⟩
 
-/-- `prefixFunction pat i …` is the maximum `k` such that `pat[0...k] = pat[stackPos - k + 1...=stackPos]`. -/
+theorem PartialMatch.isValidForSlice {pat s : Slice} (hpat : pat.isEmpty = false)
+    {pos : Pos.Raw}
+    (h : PartialMatch pat.copy.toByteArray s.copy.toByteArray pat.utf8ByteSize pos.byteIdx)
+    (h' : (pos.unoffsetBy pat.rawEndPos).IsValidForSlice s) : pos.IsValidForSlice s := by
+  have : pos.byteIdx = (s.pos _ h').offset.byteIdx + pat.copy.toByteArray.size := by
+    have := h.needlePos_le_stackPos
+    simp at ⊢ this
+    omega
+  have h₀ : pos = (pos.unoffsetBy pat.rawEndPos).increaseBy pat.utf8ByteSize := by
+    simpa [Pos.Raw.ext_iff] using this
+  rw [this, utf8ByteSize_eq_size_toByteArray_copy, ← matchesAt_iff_partialMatch hpat,
+    matchesAt_iff_isLongestMatchAt hpat] at h
+  obtain ⟨h, -⟩ := h
+  rwa [h₀]
+
+theorem PartialMatch.isLongestMatchAt
+    {pat s : Slice} (hpat : pat.isEmpty = false)
+    {pos : Pos.Raw}
+    (h : PartialMatch pat.copy.toByteArray s.copy.toByteArray pat.utf8ByteSize pos.byteIdx)
+    (h' : (pos.unoffsetBy pat.rawEndPos).IsValidForSlice s) :
+    IsLongestMatchAt pat (s.pos _ h') (s.pos _ (h.isValidForSlice hpat h')) := by
+  have : pos.byteIdx = (s.pos _ h').offset.byteIdx + pat.copy.toByteArray.size := by
+    have := h.needlePos_le_stackPos
+    simp at ⊢ this
+    omega
+  have h₀ : pos = (pos.unoffsetBy pat.rawEndPos).increaseBy pat.utf8ByteSize := by
+    simpa [Pos.Raw.ext_iff] using this
+  rw [this, utf8ByteSize_eq_size_toByteArray_copy, ← matchesAt_iff_partialMatch hpat,
+    matchesAt_iff_isLongestMatchAt hpat] at h
+  conv in s.pos pos _ => simp +singlePass [h₀]
+  exact h.2
+
+/--
+`prefixFunction pat i …` is the maximum `k` such that `pat[0...k] = pat[stackPos - k + 1...=stackPos]`.
+
+Using the implementation given here, computing a table of `prefixFunction pat i` for `i` in
+`0...pat.size` would take cubic time, but we will later show that the `buildTable` function, which
+runs in linear time, also computes this table.
+-/
 def prefixFunction (pat : ByteArray) (stackPos : Nat) (hst : stackPos < pat.size) : Nat :=
-  go (stackPos + 1)
+  go stackPos
 where go (k : Nat) : Nat :=
   if h : PartialMatch pat pat k (stackPos + 1) then
     k
@@ -108,29 +157,173 @@ theorem prefixFunction.le_go_iff {pat : ByteArray} {stackPos : Nat} {hst : stack
     exact ⟨k'', h₀, by omega, h₂⟩
 
 theorem le_prefixFunction_iff {pat : ByteArray} {stackPos : Nat} {hst : stackPos < pat.size} :
-    k ≤ prefixFunction pat stackPos hst ↔ ∃ k', k ≤ k' ∧ PartialMatch pat pat k' (stackPos + 1) := by
+    k ≤ prefixFunction pat stackPos hst ↔ ∃ k', k ≤ k' ∧ k' ≤ stackPos ∧ PartialMatch pat pat k' (stackPos + 1) := by
   rw [prefixFunction, prefixFunction.le_go_iff]
-  exact ⟨fun ⟨k', h₀, h₁, h₂⟩ => ⟨k', h₀, h₂⟩,
-    fun ⟨k', h₀, h₁⟩ => ⟨k', h₀, h₁.needlePos_le_stackPos, h₁⟩⟩
 
 theorem prefixFunction_le_iff {pat : ByteArray} {stackPos : Nat} {hst : stackPos < pat.size} :
-    prefixFunction pat stackPos hst ≤ k ↔ ∀ k', k < k' → ¬ PartialMatch pat pat k' (stackPos + 1) := by
+    prefixFunction pat stackPos hst ≤ k ↔ ∀ k', k < k' → k' ≤ stackPos → ¬ PartialMatch pat pat k' (stackPos + 1) := by
   rw [Nat.le_iff_lt_add_one, ← Std.not_le, le_prefixFunction_iff]
   simp [Nat.le_iff_lt_add_one]
 
 theorem prefixFunction_eq_iff {pat : ByteArray} {stackPos : Nat} {hst : stackPos < pat.size} :
     prefixFunction pat stackPos hst = k ↔
-      PartialMatch pat pat k (stackPos + 1) ∧ ∀ k', k < k' → ¬ PartialMatch pat pat k' (stackPos + 1) := by
-  rw [← Std.le_antisymm_iff, le_prefixFunction_iff, prefixFunction_le_iff, and_comm, and_congr_left_iff]
-  refine fun h => ⟨fun ⟨k', h₀, h₁⟩ => ?_, fun h => ⟨_, Nat.le_refl _, h⟩⟩
+      k ≤ stackPos ∧ PartialMatch pat pat k (stackPos + 1) ∧ ∀ k', k < k' → k' ≤ stackPos → ¬ PartialMatch pat pat k' (stackPos + 1) := by
+  rw [← Std.le_antisymm_iff, le_prefixFunction_iff, prefixFunction_le_iff, and_comm, ← and_assoc, and_congr_left_iff]
+  refine fun h => ⟨fun ⟨k', h₀, h₁, h₂⟩ => ⟨by omega, ?_⟩, fun ⟨h'₁, h'₂⟩ => ⟨_, Nat.le_refl _, h'₁, h'₂⟩⟩
   suffices ¬ k < k' by (obtain rfl : k = k' := by omega); assumption
-  exact fun h' => h _ h' h₁
+  exact fun h' => h _ h' h₁ h₂
 
 theorem PartialMatch.le_prefixFunction {pat : ByteArray} {stackPos needlePos : Nat}
-    (h : PartialMatch pat pat needlePos stackPos) (h₀ : 0 < stackPos) :
+    (h : PartialMatch pat pat needlePos stackPos) (h₀ : 0 < stackPos) (h₁ : needlePos ≤ stackPos - 1) :
     needlePos ≤ prefixFunction pat (stackPos - 1) (by have := h.stackPos_le_size; omega) := by
   rw [le_prefixFunction_iff]
-  exact ⟨needlePos, Nat.le_refl _, by rwa [Nat.sub_add_cancel (by omega)]⟩
+  exact ⟨needlePos, Nat.le_refl _, h₁, by rwa [Nat.sub_add_cancel (by omega)]⟩
+
+theorem partialMatch_prefixFunction (pat : ByteArray) (stackPos : Nat) (hst) :
+    PartialMatch pat pat (prefixFunction pat stackPos hst) (stackPos + 1) :=
+  (prefixFunction_eq_iff.1 rfl).2.1
+
+theorem partialMatch_prefixFunction_sub_one {pat : ByteArray} {stackPos : Nat} {hst} (h : 0 < stackPos) :
+    PartialMatch pat pat (prefixFunction pat (stackPos - 1) hst) stackPos := by
+  rw (occs := [2]) [(by omega : stackPos = stackPos - 1 + 1)]
+  exact partialMatch_prefixFunction ..
+
+theorem prefixFunction_le {pat : ByteArray} {stackPos : Nat} {hst} :
+    prefixFunction pat stackPos hst ≤ stackPos :=
+  (prefixFunction_eq_iff.1 rfl).1
+
+theorem prefixFunction_sub_one_lt {pat : ByteArray} {stackPos : Nat} {hst} (h : 0 < stackPos) :
+    prefixFunction pat (stackPos - 1) hst < stackPos := by
+  have := prefixFunction_le (hst := hst)
+  omega
+
+theorem prefixFunction_le_prefixFunction_sub_one_add_one {pat : ByteArray} {stackPos : Nat} {hst} (h₀ : 0 < stackPos) :
+    prefixFunction pat stackPos hst ≤ prefixFunction pat (stackPos - 1) (by omega) + 1 := by
+  rw [prefixFunction_le_iff]
+  refine fun k hk hk' hpart => ?_
+  rw [(by omega : k = k - 1 + 1), partialMatch_add_one_add_one_iff] at hpart
+  have := hpart.1.le_prefixFunction h₀ (by omega)
+  omega
+
+/--
+This is an implementation of `prefixFunction` that follows the efficient procedure employed by
+the `buildTable` function.
+-/
+def prefixFunctionRecurrence (pat : ByteArray) (stackPos : Nat) (hst : stackPos < pat.size)
+    (guess : Nat) (hg : guess < stackPos) : Nat :=
+  if pat[guess] = pat[stackPos] then
+    guess + 1
+  else if h : guess = 0 then
+    0
+  else
+    have : (prefixFunction pat (guess - 1) (by omega)) < guess := by
+      have := prefixFunction_le (pat := pat) (stackPos := guess - 1) (hst := by omega)
+      omega
+    prefixFunctionRecurrence pat stackPos hst (prefixFunction pat (guess - 1) (by omega)) (by omega)
+
+@[simp]
+theorem prefixFunction_zero {b hi} : prefixFunction b 0 hi = 0 :=
+  Nat.le_zero.1 prefixFunction_le
+
+theorem prefixFunctionRecurrence_eq_prefixFunction {pat : ByteArray} {stackPos : Nat} {hst : stackPos < pat.size}
+    {guess : Nat} {hg : guess < stackPos} (h : prefixFunction pat stackPos (by omega) ≤ guess + 1)
+    (hpa : PartialMatch pat pat guess stackPos) :
+    prefixFunctionRecurrence pat stackPos hst guess hg = prefixFunction pat stackPos hst := by
+  fun_induction prefixFunctionRecurrence with
+  | case1 g hg heq =>
+    refine Std.le_antisymm (le_prefixFunction_iff.2 ⟨g + 1, Nat.le_refl _, by omega, ?_⟩) h
+    exact partialMatch_add_one_add_one_iff.2 ⟨hpa, ⟨_, _, heq⟩⟩
+  | case2 hg h' =>
+    simp only [eq_comm (a := 0)]
+    suffices prefixFunction pat stackPos hst ≠ 1 by omega
+    intro heq
+    rw [prefixFunction_eq_iff] at heq
+    simp [heq.2.1.getElem_eq 0 Nat.zero_lt_one] at h'
+  | case3 g hg heq hg₀ hlt ih =>
+    apply ih
+    · simp only [prefixFunction_le_iff]
+      refine fun k h hk' hpart => ?_
+      have hpx := hpart.le_prefixFunction (by omega) (by omega)
+      simp only [Nat.add_one_sub_one] at hpx
+      rw [(by omega : k = k - 1 + 1), partialMatch_add_one_add_one_iff] at hpart
+      obtain ⟨hp₁, ⟨_, _, hp₂⟩⟩ := hpart
+      have := hpa.partialMatch_iff.2 ⟨by omega, hp₁⟩
+      have := this.le_prefixFunction (by omega)
+      suffices k - 1 ≠ g by omega
+      rintro rfl
+      simp [hp₂] at heq
+    · exact (hpa.partialMatch_iff.1 (partialMatch_prefixFunction_sub_one (by omega))).2
+
+/-- Predicate that an array is a correct precomputation of the prefix function. -/
+structure IsTable (b : ByteArray) (v : Array Nat) : Prop where
+  size_le : v.size ≤ b.size
+  eq_prefixFunction (i : Nat) (hi) : v[i]'hi = prefixFunction b i (by omega)
+
+@[simp]
+theorem isTable_empty : IsTable ByteArray.empty #[] where
+  size_le := by simp
+  eq_prefixFunction := by simp
+
+theorem isTable_singleton {b : ByteArray} (hb : 1 ≤ b.size) : IsTable b #[0] where
+  size_le := by simp [hb]
+  eq_prefixFunction := by simp +contextual
+
+theorem IsTable.push {b : ByteArray} {v : Array Nat} (h : IsTable b v) {d : Nat}
+    (hle : v.size + 1 ≤ b.size)
+    (hd : d = prefixFunction b v.size (by omega)) :
+    IsTable b (v.push d) where
+  size_le := by simpa using hle
+  eq_prefixFunction i hi := by
+    rw [Array.getElem_push]
+    split <;> rename_i hi'
+    · rw [h.eq_prefixFunction]
+    · rw [Array.size_push] at hi
+      obtain rfl : i = v.size := by omega
+      exact hd
+
+theorem computeDistance_eq_prefixFunctionRecurrence {s : Slice} (i : Nat)
+    (hi : i < s.copy.toByteArray.size) {patByte : UInt8}
+    (hpat : patByte = s.copy.toByteArray[i])
+    (table : Array Nat) {ht} (ht' : IsTable s.copy.toByteArray table) {h guess hg hg'} :
+    (buildTable.computeDistance s patByte table ht h guess hg').1 =
+      prefixFunctionRecurrence s.copy.toByteArray i (by omega) guess hg := by
+  cases hpat
+  fun_induction prefixFunctionRecurrence with
+  | case1 =>
+    rw [buildTable.computeDistance, if_pos]
+    simp [getUTF8Byte_eq_getUTF8Byte_copy, String.getUTF8Byte, *]
+  | case2 =>
+    rw [buildTable.computeDistance, if_neg, dif_pos]
+    · rfl
+    · simp [getUTF8Byte_eq_getUTF8Byte_copy, String.getUTF8Byte, *]
+  | case3 g hg h₁ h₂ h₃ ih =>
+    rw [buildTable.computeDistance, if_neg, dif_neg h₂]
+    · simp only [ht'.eq_prefixFunction, ih]
+    · simp [getUTF8Byte_eq_getUTF8Byte_copy, String.getUTF8Byte, *]
+
+theorem isTable_buildTableGo {pat : Slice} {table : Array Nat} {ht₀ ht h} (ht' : IsTable pat.copy.toByteArray table) :
+    IsTable pat.copy.toByteArray (buildTable.go pat table ht₀ ht h).1 := by
+  fun_induction buildTable.go with
+  | case1 t ht₀ ht h hlt patByte dist ih =>
+    refine ih (ht'.push (by simp; omega) ?_)
+    simp only [getUTF8Byte_eq_getUTF8Byte_copy, String.getUTF8Byte, ht'.eq_prefixFunction, dist,
+      patByte]
+    rw [computeDistance_eq_prefixFunctionRecurrence _ _ rfl _ ht', prefixFunctionRecurrence_eq_prefixFunction]
+    · exact prefixFunction_le_prefixFunction_sub_one_add_one ht₀
+    · exact partialMatch_prefixFunction_sub_one ht₀
+    · exact prefixFunction_sub_one_lt ht₀
+  | case2 t ht₀ ht h hlt => simpa
+
+theorem isTable_buildTable {pat : Slice} : IsTable pat.copy.toByteArray (buildTable pat).toArray := by
+  rw [buildTable]
+  split
+  · simp [String.toByteArray_eq_empty_iff.2 (by rwa [Slice.copy_eq_empty_iff, Slice.isEmpty_iff])]
+  · exact isTable_buildTableGo (by simpa using isTable_singleton (by simp; omega))
+
+@[simp]
+theorem getElem_buildTable {pat : Slice} {i hi} :
+    (buildTable pat)[i]'hi = prefixFunction pat.copy.toByteArray i (by simpa) := by
+  rw [← Vector.getElem_toArray (h := by simpa), isTable_buildTable.eq_prefixFunction]
 
 /--
 These are the invariants satisfied by the KMP search iterator. They are sufficient to ensure that
@@ -139,40 +332,211 @@ the code does not panic and returns the correct result.
 structure Invariants (pat s : Slice) (needlePos stackPos : String.Pos.Raw) : Prop where
   isEmpty_eq_false : pat.isEmpty = false
   partialMatch : PartialMatch pat.copy.toByteArray s.copy.toByteArray needlePos.byteIdx stackPos.byteIdx
-  isValid : (stackPos.unoffsetBy needlePos).IsValidForSlice s
+  isValidForSlice' : needlePos = 0 → stackPos.IsValidForSlice s
 
-/-
-theorem PartialMatch.partialMatch_iff {pat s : ByteArray} {stackPos needlePos : Nat}
-    (h : PartialMatch pat s needlePos stackPos) {needlePos' : Nat} :
-    PartialMatch pat pat needlePos' needlePos ↔
-      needlePos' ≤ needlePos ∧ PartialMatch pat s needlePos' stackPos := by
--/
+theorem Invariants.inc {pat s : Slice} {stackPos needlePos : String.Pos.Raw} (h₀ : Invariants pat s needlePos stackPos)
+    (h₁ h₂)
+    (h : pat.getUTF8Byte needlePos h₁ = s.getUTF8Byte stackPos h₂) : Invariants pat s needlePos.inc stackPos.inc where
+  isEmpty_eq_false := h₀.isEmpty_eq_false
+  partialMatch := partialMatch_add_one_add_one_iff.2 ⟨h₀.partialMatch, ⟨_, _,
+    by simpa [getUTF8Byte_eq_getUTF8Byte_copy, String.getUTF8Byte] using h⟩⟩
+  isValidForSlice' := by simp
+
+theorem Invariants.isValidForSlice {pat s : Slice} {needlePos stackPos : String.Pos.Raw}
+    (h : Invariants pat s needlePos stackPos) : (stackPos.unoffsetBy needlePos).IsValidForSlice s := by
+  by_cases hn : needlePos = 0
+  · cases hn
+    simpa using h.isValidForSlice' rfl
+  · simp only [Pos.Raw.ext_iff, Pos.Raw.byteIdx_zero] at hn
+    rw [Pos.Raw.isValidForSlice_iff_isUTF8FirstByte, Classical.or_iff_not_imp_left]
+    intro hst
+    refine ⟨?_, ?_⟩
+    · have := h.partialMatch.stackPos_le_size
+      simp only [Pos.Raw.ext_iff, Pos.Raw.byteIdx_unoffsetBy, byteIdx_rawEndPos, size_toByteArray,
+        utf8ByteSize_copy, Pos.Raw.lt_iff, gt_iff_lt] at ⊢ hst this
+      omega
+    · simp only [getUTF8Byte_eq_getUTF8Byte_copy, String.getUTF8Byte, Pos.Raw.byteIdx_unoffsetBy]
+      simp +singlePass only [← Nat.add_zero (stackPos.byteIdx - needlePos.byteIdx),
+        ← h.partialMatch.getElem_eq 0 (by omega)]
+      exact pat.copy.isValidUTF8.isUTF8FirstByte_getElem_zero ..
+
+theorem Invariants.offset {pat s : Slice} {pos : s.Pos} (hpat : pat.isEmpty = false) :
+    Invariants pat s 0 pos.offset where
+  isEmpty_eq_false := hpat
+  partialMatch := partialMatch_zero (by simpa [Pos.Raw.le_iff, Pos.le_iff] using pos.le_endPos)
+  isValidForSlice' _ := pos.isValidForSlice
+
+/-- The start of the window, as a valid position in `s.` -/
+def Invariants.base {pat s : Slice} {needlePos stackPos : String.Pos.Raw}
+    (h : Invariants pat s needlePos stackPos) : s.Pos :=
+  s.pos _ h.isValidForSlice
+
+theorem Invariants.zero_of_eq {pat s : Slice} {stackPos needlePos : String.Pos.Raw}
+    (h : Invariants pat s needlePos stackPos) (h' : needlePos = pat.rawEndPos) :
+    Invariants pat s 0 stackPos := by
+  cases h'
+  refine ⟨h.isEmpty_eq_false, partialMatch_zero h.partialMatch.stackPos_le_size, fun _ => ?_⟩
+  exact h.partialMatch.isValidForSlice h.isEmpty_eq_false h.isValidForSlice
+
+theorem Invariants.isLongestMatchAt {pat s : Slice} {stackPos needlePos : String.Pos.Raw}
+    (h : Invariants pat s needlePos stackPos) (h' : needlePos = pat.rawEndPos) :
+    IsLongestMatchAt pat h.base (h.zero_of_eq h').base := by
+  cases h'
+  exact h.partialMatch.isLongestMatchAt h.isEmpty_eq_false h.isValidForSlice
 
 theorem Invariants.not_matchesAt_of_prefixFunction_eq {pat s : Slice} {stackPos needlePos : String.Pos.Raw}
     (h : Invariants pat s needlePos stackPos)
-    (h' : 0 < needlePos) {k : Nat} {hki} (hk : prefixFunction pat.copy.toByteArray (needlePos.byteIdx - 1) hki = k)
+    {k : Nat} {hki} (hk : prefixFunction pat.copy.toByteArray (needlePos.byteIdx - 1) hki = k)
     (p : s.Pos) (hp₁ : stackPos.unoffsetBy needlePos ≤ p.offset) (hp₂ : p.offset < stackPos.unoffsetBy ⟨k⟩)
-    -- {h₁ h₂}
-    -- (hmism : s.getUTF8Byte stackPos h₁ ≠ pat.getUTF8Byte needlePos h₂)
-    :
+    {h₁ h₂} (hmism : s.getUTF8Byte stackPos h₁ ≠ pat.getUTF8Byte needlePos h₂) :
     ¬ MatchesAt pat p := by
-  -- simp [getUTF8Byte_eq_getUTF8Byte_copy, String.getUTF8Byte] at hmism
+  simp only [getUTF8Byte_eq_getUTF8Byte_copy, String.getUTF8Byte, ne_eq] at hmism
   rw [matchesAt_iff_partialMatch h.isEmpty_eq_false]
   intro hpart
-  simp only [Pos.Raw.le_iff, Pos.Raw.byteIdx_unoffsetBy, Nat.sub_le_iff_le_add, Pos.Raw.lt_iff,
-    Pos.Raw.byteIdx_zero] at hp₁ hp₂ h'
-  have := hpart.partialMatch_of_le stackPos.byteIdx (by omega) (by omega)
-  have := hk ▸ (h.partialMatch.partialMatch_iff.2 ⟨by omega, this⟩).le_prefixFunction h'
-  omega
+  simp only [Pos.Raw.le_iff, Pos.Raw.byteIdx_unoffsetBy, Nat.sub_le_iff_le_add, Pos.Raw.lt_iff] at hp₁ hp₂
+  by_cases hin : stackPos.byteIdx - p.offset.byteIdx ≤ needlePos.byteIdx - 1
+  · have := hpart.partialMatch_of_le stackPos.byteIdx (by omega) (by omega)
+    have := hk ▸ (h.partialMatch.partialMatch_iff.2 ⟨by omega, this⟩).le_prefixFunction (by omega) (by omega)
+    omega
+  · obtain rfl : stackPos = needlePos.offsetBy p.offset := by simpa [Pos.Raw.ext_iff] using by omega
+    simp [hpart.getElem_eq needlePos.byteIdx (by simpa [Pos.Raw.lt_iff] using h₂)] at hmism
 
--- def prefixFunction (b : ByteArray) (i : Nat) (hi : i < b.size) : Nat :=
---   go i
--- where go (k : Nat) : Nat :=
---   if h : PartialMatch b i hi k then
---     k
---   else
---     have : k ≠ 0 := by rintro rfl; simp_all
---     go (k - 1)
+theorem Invariants.of_prefixFunction_eq {pat s : Slice} {stackPos needlePos : String.Pos.Raw}
+    (h : Invariants pat s needlePos stackPos)
+    (h' : needlePos ≠ 0) {k : Nat} {hki}
+    (hk : prefixFunction pat.copy.toByteArray (needlePos.byteIdx - 1) hki = k) (hk₀ : 0 < k) :
+    Invariants pat s ⟨k⟩ stackPos := by
+  refine ⟨h.isEmpty_eq_false, ?_, by simp [Nat.pos_iff_ne_zero.1 hk₀]⟩
+  have := partialMatch_prefixFunction (hst := hki)
+  rw [Nat.sub_add_cancel (by simp at h'; omega)] at this
+  exact hk ▸ (h.partialMatch.partialMatch_iff.1 this).2
+
+theorem Invariants.isValidSearchFrom_toList {pat s : Slice} {stackPos needlePos : String.Pos.Raw}
+    (it : Std.Iter (α := ForwardSliceSearcher s) (SearchStep s))
+    (h : Invariants pat s needlePos stackPos)
+    {table ht hn}
+    (heq : it = Std.Iter.mk (.proper pat table ht stackPos needlePos hn))
+    {p : s.Pos} (hp : p = h.base) :
+    IsValidSearchFrom pat p it.toList := by
+  induction it using Std.Iter.inductSteps generalizing p stackPos needlePos with | step it ihy ihs
+  cases heq
+  cases hp
+  rw [Std.Iter.toList_eq_match_step]
+  generalize hit' : (Std.Iter.mk (α := ForwardSliceSearcher s)
+    (.proper pat table ht stackPos needlePos hn)).step = it'
+
+  have hit'' := congrArg Subtype.val hit'
+  have plausible := it'.property
+  simp only [Std.Iter.step_eq, ne_eq, Std.Iter.toIterM] at hit''
+  split at hit'' <;> rename_i h₁
+  · split at hit'' <;> rename_i h₂
+    · split at hit'' <;> rename_i h₃
+      · -- Case 1: matched the full pattern
+        simp only [Id.run_pure, Std.Shrink.inflate_deflate, Std.IterM.Step.toPure_yield,
+          Std.PlausibleIterStep.yield, Std.IterM.toIter_mk] at hit''
+        have hinc := h.inc _ _ h₂.symm
+        have hzero := hinc.zero_of_eq h₃
+        rw [s.pos!_eq_pos hinc.isValidForSlice, s.pos!_eq_pos (hzero.isValidForSlice' rfl)] at hit''
+        simp only [← hit'', Pos.Raw.inc_unoffsetBy_inc] at ⊢ plausible
+        apply IsValidSearchFrom.matched_of_eq (ihy plausible hzero rfl rfl) _ rfl
+        simpa [base] using hinc.isLongestMatchAt h₃
+
+      · -- Case 2: matched the next character, but not yet the full pattern
+        simp only [Id.run_pure, Std.Shrink.inflate_deflate, Std.IterM.Step.toPure_skip,
+          Std.PlausibleIterStep.skip, Std.IterM.toIter_mk] at hit''
+        simp only [← hit''] at ⊢ plausible
+        exact ihs plausible (h.inc _ _ h₂.symm) rfl (by simp [base])
+
+    · split at hit'' <;> rename_i h₃
+      · -- Case 3: mismatch at the start of the pattern -> jump to next position
+        simp only [Id.run_pure, Std.Shrink.inflate_deflate, Std.IterM.Step.toPure_yield,
+          Std.PlausibleIterStep.yield, Std.IterM.toIter_mk] at hit''
+        cases h₃
+        rw [s.pos!_eq_pos (h.isValidForSlice' rfl)] at hit''
+        simp only [← hit''] at ⊢ plausible
+        apply IsValidSearchFrom.mismatched_of_eq _ (by simp [base]) _ (by simp [base])
+        · exact ihy plausible (.offset h.isEmpty_eq_false) rfl rfl
+        · simp only [base, Pos.Raw.unoffsetBy_zero, Pos.le_iff, offset_pos, lt_posGT_iff]
+          intro pos hp₁ hp₂
+          obtain rfl : stackPos = pos.offset := Std.le_antisymm hp₁ hp₂
+          simpa [matchesAt_iff_getElem h.isEmpty_eq_false] using fun h => ⟨0, by simpa,
+            by simpa [getUTF8Byte_eq_getUTF8Byte_copy, String.getUTF8Byte] using Ne.symm h₂⟩
+
+      · cases ht
+        simp only [getElem_buildTable] at hit''
+
+        split at hit'' <;> rename_i h₄
+        · -- Case 4: mismatch in the middle of the pattern, and no common prefix ->
+          -- jump to next position if not at the start of the character
+          simp only [Id.run_pure, Std.Shrink.inflate_deflate, Std.IterM.Step.toPure_yield,
+            Std.PlausibleIterStep.yield, Std.IterM.toIter_mk] at hit''
+          rw [s.pos!_eq_pos h.isValidForSlice] at hit''
+          simp only [← hit''] at ⊢ plausible
+          apply IsValidSearchFrom.mismatched_of_eq _ _ _ (by simp [base])
+          · exact ihy plausible (.offset h.isEmpty_eq_false) rfl rfl
+          · have := h.partialMatch.needlePos_le_stackPos
+            simp only [Pos.Raw.ext_iff, Pos.Raw.byteIdx_zero, base, lt_posGE_iff, offset_pos,
+              Pos.Raw.lt_iff, Pos.Raw.byteIdx_unoffsetBy, gt_iff_lt] at ⊢ h₃
+            omega
+          · simp only [base, lt_posGE_iff]
+            exact fun p hp₁ hp₂ => not_matchesAt_of_prefixFunction_eq h h₄ _ hp₁ hp₂ h₂
+
+        · -- Case 5: mismatch in the middle of the pattern with a common prefix
+          simp only [Id.run_pure, Std.Shrink.inflate_deflate, Std.IterM.Step.toPure_yield,
+            Std.PlausibleIterStep.yield, Std.IterM.toIter_mk] at hit''
+          rw [s.pos!_eq_pos h.isValidForSlice,
+            s.pos!_eq_pos (h.of_prefixFunction_eq h₃ rfl (by omega)).isValidForSlice] at hit''
+          simp only [← hit''] at ⊢ plausible
+          apply IsValidSearchFrom.mismatched_of_eq _ _ _ (by simp [base])
+          · exact ihy plausible (h.of_prefixFunction_eq h₃ rfl (by omega)) rfl rfl
+          · have h₅ := h.partialMatch.needlePos_le_stackPos
+            simp [base, Pos.lt_iff, Pos.Raw.ext_iff] at ⊢ h₃ h₅
+            apply Pos.Raw.unoffsetBy_lt_unoffsetBy_of_le_of_lt
+            all_goals exact Std.lt_of_le_of_lt prefixFunction_le (by simp [Pos.Raw.lt_iff]; omega)
+          · exact fun p hp₁ hp₂ => not_matchesAt_of_prefixFunction_eq h rfl _ hp₁ hp₂ h₂
+
+  · split at hit'' <;> rename_i h₂
+    · -- Case 6: so close to the end that we cannot match anymore -> reject, then done
+      simp only [Id.run_pure, Std.Shrink.inflate_deflate, Std.IterM.Step.toPure_yield,
+        Std.PlausibleIterStep.yield, Std.IterM.toIter_mk] at hit''
+      rw [s.pos!_eq_pos h.isValidForSlice] at hit''
+      simp only [← hit''] at ⊢ plausible
+      apply IsValidSearchFrom.mismatched_of_eq _ _ _ (by simp [base])
+      · rw [Std.Iter.toList_eq_match_step, Std.Iter.step_eq]
+        simpa [Std.Iter.toIterM] using IsValidSearchFrom.endPos
+      · simp only [Pos.Raw.lt_iff, Pos.Raw.byteIdx_unoffsetBy, byteIdx_rawEndPos, base, Pos.lt_iff,
+          offset_pos, offset_endPos] at ⊢ h₂
+        omega
+      · refine fun p hp₁ hp₂ hm => ?_
+        have := le_of_matchesAt h.isEmpty_eq_false hm
+        simp only [base, Pos.le_iff, offset_pos, Pos.Raw.le_iff, Pos.Raw.byteIdx_unoffsetBy,
+          Nat.sub_le_iff_le_add, Pos.Raw.byteIdx_increaseBy, byteIdx_rawEndPos,
+          Nat.not_le] at hp₁ this h₁
+        omega
+
+    · --  Case 7: reached the end with empty partial match -> done
+      simp only [base, ← hit'', Id.run_pure, Std.Shrink.inflate_deflate, Std.IterM.Step.toPure_done,
+        Std.PlausibleIterStep.done, Std.IterM.toIter_mk]
+      apply IsValidSearchFrom.endPos_of_eq (Std.le_antisymm (Pos.le_endPos _) _) rfl
+      simpa [Pos.Raw.le_iff, Pos.le_iff, Pos.Raw.lt_iff] using h₂
+
+theorem Invariants.start (pat s : Slice) (h : pat.isEmpty = false) :
+    Invariants pat s 0 0 where
+  isEmpty_eq_false := h
+  partialMatch := partialMatch_zero (by simp)
+  isValidForSlice' := by simp
+
+theorem Invariants.base_start {pat s : Slice} (h : pat.isEmpty = false) :
+    (Invariants.start pat s h).base = s.startPos :=
+  rfl
+
+public theorem lawfulToForwardSearcherModel {pat : Slice} (hpat : pat.isEmpty = false) :
+    LawfulToForwardSearcherModel pat where
+  isValidSearchFrom_toList s := by
+    simp only [ToForwardSearcher.toSearcher]
+    rw [iter, dif_neg (by simpa [isEmpty_eq] using hpat)]
+    rw (occs := [1]) [← Invariants.base_start hpat]
+    apply Invariants.isValidSearchFrom_toList _ _ rfl rfl
 
 end ForwardSliceSearcher
 
