src/Init/Data/String/Lemmas/Basic.lean
@@ -163,4 +163,9 @@ theorem cast_pos {s t : String} {p : Pos.Raw} {h : Pos.Raw.IsValid s p} {h' : s 
     (s.pos p h).cast h' = t.pos p (h' ▸ h) := by
   simp [String.Pos.ext_iff]
 
+@[simp]
+theorem Pos.Raw.isValidForSlice_zero {s : Slice} : (0 : Pos.Raw).IsValidForSlice s where
+  le_rawEndPos := by simp [Pos.Raw.le_iff]
+  isValid_offsetBy := by simpa using s.startInclusive.isValid
+
 end String
