src/Init/Data/String/Lemmas/Pattern/String/Basic.lean
@@ -117,6 +117,10 @@ theorem matchesAt_iff_getElem {pat s : Slice} {pos : s.Pos} (h : pat.isEmpty = f
       omega
     · simp [ByteArray.getElem_extract, h₂]
 
+theorem le_of_matchesAt {pat s : Slice} {pos : s.Pos} (h : pat.isEmpty = false)
+    (h' : MatchesAt pat pos) : pos.offset.increaseBy pat.utf8ByteSize ≤ s.rawEndPos := by
+  simpa [Pos.Raw.le_iff] using ((matchesAt_iff_getElem h).1 h').1
+
 -- TODO: clean up this proof
 -- theorem matchesAt_iff_extract {pat s : Slice} {pos : s.Pos} (h : pat.isEmpty = false) :
 --     MatchesAt pat pos ↔
